\documentclass[journal,12pt,twocolumn]{IEEEtran}

\usepackage{enumitem}
\usepackage{tfrupee}
\usepackage{amsmath}
\usepackage{amssymb}
\usepackage{gensymb}
\usepackage{graphicx}
\usepackage{txfonts}

\def\inputGnumericTable{}

\usepackage[latin1]{inputenc}
\usepackage{color}
\usepackage{array}
\usepackage{longtable}
\usepackage{calc}
\usepackage{multirow}
\usepackage{hhline}
\usepackage{ifthen}
\providecommand{\pr}[1]{\ensuremath{\Pr\left(#1\right)}}
\providecommand{\cbrak}[1]{\ensuremath{\left\{#1\right\}}}
\renewcommand{\thefigure}{\arabic{table}}
\renewcommand{\thetable}{\arabic{table}}
\title{Assignment 7 \\ \Large AI1110: Probability and Random Variables \\ \large Indian Institute of Technology Hyderabad}
\author{Rudransh Mishra \\ \normalsize AI21BTECH11025 \\ \vspace*{20pt} \normalsize  15 June 2022 \\ \vspace*{20pt} PROBABILITY, RANDOM VARIABLES, AND STOCHASTIC PROCESSES\\ \normalsize Athanasios Papoulis}

\begin{document}
% The title
\maketitle

% The question
% The question
\textbf{Example 15.2}
Suppose-that s[n] is a first-order AR process and v[n] is white noise orthogonal to s[n]:
\begin{align}
& S_ss (z) = $\(\frac{N_0}{(1 - az^{-1})(l - az)}\)$\\
& S_vv (z) = N \\
& S_sv (z) = 0
\end{align}

In this case,
\begin{align}
S_xx (z) = S_ss (z) + N = \frac{aN(l - bz^{-1} )(1 - bz)}{b(1- az^{-1})(1- az)}
\end{align}
where $0<b<a<1$ and $b+b^{-1}=a+a^{-1}$ + $\frac{N_0}{aN}$

Hence\\
\begin{align}
& H(z)=$\(\frac{bN_0}{aN(1 - bz^-1)(1 - bz)}\)$\\
& h[n] = cb^{|n|}\\$
& c=\(\frac{bN_0}{aN(1- b^2)}\)$\\
& P=$\(\frac{bNo}{1 - a^2}\)[1- c\sum_{k=-\infty}^{k=\infty}(ab)^{|k|}]\\ $
& P=$\(\frac{bN_0}{a(1-b_2)}\)$
\end{align}

\begin{center} ---x-x-x-x-x-x--- \end{center}
\end{document}
